src/HaskStrongToProof.v
@@ -56,13 +56,11 @@ Definition copyAndPivotContext {Γ}{Δ} a b c τ :
 Context {VV:Type}{eqd_vv:EqDecidable VV}.
 
   (* maintenance of Xi *)
-  Definition dropVar (lv:list VV)(v:VV) : ??VV :=
-    if fold_left
-      (fun a b:bool => if a then true else if b then true else false)
-      (map (fun lvv => if eqd_dec lvv v then true else false) lv)
-      false
-      then None
-      else Some v.
+  Fixpoint dropVar (lv:list VV)(v:VV) : ??VV :=
+    match lv with
+      | nil     => Some v
+      | v'::lv' => if eqd_dec v v' then None else dropVar lv' v
+    end.
   (* later: use mapOptionTreeAndFlatten *)
   Definition stripOutVars (lv:list VV) : Tree ??VV -> Tree ??VV :=
     mapTree (fun x => match x with None => None | Some vt => dropVar lv vt end).
@@ -104,7 +102,7 @@ end
 with eLetRecContext {Γ}{Δ}{ξ}{lev}{tree}(elrb:ELetRecBindings Γ Δ ξ lev tree) : Tree ??VV :=
 match elrb with
   | ELR_nil    Γ Δ ξ lev  => []
-  | ELR_leaf   Γ Δ ξ lev v e => expr2antecedent e
+  | ELR_leaf   Γ Δ ξ lev v t e => expr2antecedent e
   | ELR_branch Γ Δ ξ lev t1 t2 b1 b2 => (eLetRecContext b1),,(eLetRecContext b2)
 end.
 
@@ -121,27 +119,28 @@ Definition mkProofCaseBranch {Γ}{Δ}{ξ}{l}{tc}{tbranches}{atypes}
      |}.
      Defined.
 
-Fixpoint eLetRecTypes {Γ}{Δ}{ξ}{lev}{τ}(elrb:ELetRecBindings Γ Δ ξ lev τ) : Tree ??(LeveledHaskType Γ ★) :=
+
+Fixpoint eLetRecTypes {Γ}{Δ}{ξ}{lev}{τ}(elrb:ELetRecBindings Γ Δ ξ lev τ) : Tree ??(HaskType Γ ★) :=
   match elrb with
   | ELR_nil    Γ Δ ξ lev  => []
-  | ELR_leaf   Γ Δ ξ  lev  v e => [ξ v]
+  | ELR_leaf   Γ Δ ξ  lev  v t e => [t]
   | ELR_branch Γ Δ ξ lev t1 t2 b1 b2 => (eLetRecTypes b1),,(eLetRecTypes b2)
   end.
-
+(*
 Fixpoint eLetRecVars {Γ}{Δ}{ξ}{lev}{τ}(elrb:ELetRecBindings Γ Δ ξ lev τ) : Tree ??VV :=
   match elrb with
   | ELR_nil    Γ Δ ξ lev  => []
-  | ELR_leaf   Γ Δ ξ  lev  v e => [v]
+  | ELR_leaf   Γ Δ ξ  lev  v _ _ e => [v]
   | ELR_branch Γ Δ ξ lev t1 t2 b1 b2 => (eLetRecVars b1),,(eLetRecVars b2)
   end.
 
-Fixpoint eLetRecTypesVars {Γ}{Δ}{ξ}{lev}{τ}(elrb:ELetRecBindings Γ Δ ξ lev τ) : Tree ??(VV * LeveledHaskType Γ ★):=
+Fixpoint eLetRecTypesVars {Γ}{Δ}{ξ}{lev}{τ}(elrb:ELetRecBindings Γ Δ ξ lev τ) : Tree ??(VV * HaskType Γ ★):=
   match elrb with
   | ELR_nil    Γ Δ ξ lev  => []
-  | ELR_leaf   Γ Δ ξ  lev  v e => [(v, ξ v)]
+  | ELR_leaf   Γ Δ ξ  lev  v t _ e => [(v, t)]
   | ELR_branch Γ Δ ξ lev t1 t2 b1 b2 => (eLetRecTypesVars b1),,(eLetRecTypesVars b2)
   end.
-
+*)
 
 Lemma stripping_nothing_is_inert
   {Γ:TypeEnv}
@@ -154,12 +153,14 @@ Lemma stripping_nothing_is_inert
     fold stripOutVars.
     simpl.
     fold (stripOutVars nil).
-    rewrite IHtree1.
-    rewrite IHtree2.
+    rewrite <- IHtree1 at 2.
+    rewrite <- IHtree2 at 2.
     reflexivity.
     Qed.
 
-
+Ltac eqd_dec_refl X :=
+  destruct (eqd_dec X X) as [eqd_dec1 | eqd_dec2];
+    [ clear eqd_dec1 | set (eqd_dec2 (refl_equal _)) as eqd_dec2'; inversion eqd_dec2' ].
 
 Definition arrangeContext 
      (Γ:TypeEnv)(Δ:CoercionEnv Γ)
@@ -179,17 +180,18 @@ Definition arrangeContext
           [Γ >> Δ > mapOptionTree ξ                         ctx                       |- τ]
           [Γ >> Δ > mapOptionTree ξ ((stripOutVars (v::nil) ctx),,[v])                |- τ]).
 
-  induction ctx; simpl in *.
+  induction ctx.
   
-    refine (match a with None => let case_None := tt in _ | Some v' => let case_Some := tt in _ end); simpl in *.
+    refine (match a with None => let case_None := tt in _ | Some v' => let case_Some := tt in _ end).
   
         (* nonempty leaf *)
         destruct case_Some.
           unfold stripOutVars in *; simpl.
           unfold dropVar.
           unfold mapOptionTree in *; simpl; fold (mapOptionTree ξ) in *.
-          destruct (eqd_dec v v'); simpl in *.
 
+          destruct (eqd_dec v' v); subst.
+          
             (* where the leaf is v *)
             apply inr.
               subst.
@@ -287,12 +289,51 @@ Definition arrangeContextAndWeaken v ctx Γ Δ τ ξ :
   refine (ext_left _ _ _ (nd_rule (RWeak _ _))).
   Defined.
 
+Lemma strip_lemma a x t : stripOutVars (a::x) t = stripOutVars (a::nil) (stripOutVars x t).
+  unfold stripOutVars.
+  rewrite <- mapTree_compose.
+  induction t; try destruct a0.
+  simpl.
+  induction x.
+    reflexivity.
+    admit.
+  subst.
+  reflexivity.
+  simpl in *.
+  rewrite <- IHt1.
+  rewrite <- IHt2.
+  reflexivity.
+  Qed.
+
+Lemma strip_twice_lemma x y t : stripOutVars x (stripOutVars y t) = stripOutVars (app y x) t.
+  induction x.
+  simpl.
+  admit.
+  rewrite strip_lemma.
+  rewrite IHx.
+  rewrite <- strip_lemma.
+  admit.
+  Qed.
+
+Lemma distinct_app1 : forall T (l1 l2:list T), distinct (app l1 l2) -> distinct l1.
+  admit.
+  Qed.
+
+Lemma distinct_app2 : forall T (l1 l2:list T), distinct (app l1 l2) -> distinct l2.
+  admit.
+  Qed.
+
+Lemma strip_distinct x y : distinct (app (leaves y) x) -> stripOutVars x y = y.
+  admit.
+  Qed.
+
 Definition arrangeContextAndWeaken'' Γ Δ ξ v : forall ctx z, 
+  distinct (leaves v) ->
   ND (@URule Γ Δ)
     [Γ >> Δ>(mapOptionTree ξ ctx)                                       |-  z]
     [Γ >> Δ>(mapOptionTree ξ (stripOutVars (leaves v) ctx)),,(mapOptionTree ξ v) |-  z].
 
-  induction v.
+  induction v; intros.
     destruct a.
     unfold mapOptionTree in *.
     simpl in *.
@@ -321,37 +362,24 @@ Definition arrangeContextAndWeaken'' Γ Δ ξ v : forall ctx z,
     simpl in IHv2'.
     fold (mapOptionTree ξ) in IHv2'.
     fold X in IHv2'.
-    set (nd_comp (IHv1 _ _) IHv2') as qq.
+    set (nd_comp (IHv1 _ _ (distinct_app1 _ _ _ H)) (IHv2' (distinct_app2 _ _ _ H))) as qq.
     eapply nd_comp.
       apply qq.
       clear qq IHv2' IHv2 IHv1.
-        
-      assert ((stripOutVars (leaves v2) (stripOutVars (leaves v1) ctx))=(stripOutVars (app (leaves v1) (leaves v2)) ctx)).
-        admit.
-        rewrite H.
-        clear H.
+      rewrite strip_twice_lemma.
 
-      (* FIXME: this only works because the variables are all distinct, but I need to prove that *)
-      assert ((stripOutVars (leaves v2) v1) = v1).
-        admit.
-        rewrite H.
-        clear H.
-
+      rewrite (strip_distinct (leaves v2) v1).
         apply nd_rule.
         apply RCossa.
+        auto.
     Defined.
 
-Definition update_ξ'' {Γ} ξ tree lev :=
-(update_ξ ξ
-                  (map (fun x : VV * HaskType Γ ★ => ⟨fst x, snd x @@  lev ⟩)
-                     (leaves tree))).
-
-Lemma updating_stripped_tree_is_inert {Γ} (ξ:VV -> LeveledHaskType Γ ★) v tree lev :
-      mapOptionTree (update_ξ ξ ((v,lev)::nil)) (stripOutVars (v :: nil) tree)
+Lemma updating_stripped_tree_is_inert {Γ} (ξ:VV -> LeveledHaskType Γ ★) v tree t lev :
+      mapOptionTree (update_ξ ξ lev ((v,t)::nil)) (stripOutVars (v :: nil) tree)
     = mapOptionTree ξ (stripOutVars (v :: nil) tree).
   induction tree; simpl in *; try reflexivity; auto.
 
-  unfold mapOptionTree in *; simpl; fold (mapOptionTree ξ) in *; fold (mapOptionTree (update_ξ ξ ((v,lev)::nil))) in *.
+  unfold mapOptionTree in *; simpl; fold (mapOptionTree ξ) in *; fold (mapOptionTree (update_ξ ξ lev ((v,t)::nil))) in *.
   destruct a; simpl; try reflexivity.
   unfold update_ξ.
   simpl.
@@ -363,6 +391,7 @@ Lemma updating_stripped_tree_is_inert {Γ} (ξ:VV -> LeveledHaskType Γ ★) v t
   assert (q=eqd_dec v v0).
     reflexivity.
   destruct q.
+(*
   reflexivity.
   rewrite <- H.
   reflexivity.
@@ -376,135 +405,77 @@ Lemma updating_stripped_tree_is_inert {Γ} (ξ:VV -> LeveledHaskType Γ ★) v t
   rewrite <- IHtree1.
   rewrite <- IHtree2.
   reflexivity.
+*)
+admit.
+admit.
+admit.
   Qed.
-
 
 
 Lemma updating_stripped_tree_is_inert'
   {Γ} lev
   (ξ:VV -> LeveledHaskType Γ ★)
   tree tree2 :
-    mapOptionTree (update_ξ'' ξ tree lev) (stripOutVars (leaves (mapOptionTree (@fst _ _) tree)) tree2)
+    mapOptionTree (update_ξ ξ lev (leaves tree)) (stripOutVars (leaves (mapOptionTree (@fst _ _) tree)) tree2)
   = mapOptionTree ξ (stripOutVars (leaves (mapOptionTree (@fst _ _) tree)) tree2).
-admit.
+  admit.
   Qed.
 
-Lemma updating_stripped_tree_is_inert''
-  {Γ}
-  (ξ:VV -> LeveledHaskType Γ ★)
-  v tree lev :
-    mapOptionTree   (update_ξ'' ξ (unleaves v) lev) (stripOutVars (map (@fst _ _) v) tree)
-  = mapOptionTree ξ (stripOutVars  (map (@fst _ _) v) tree).
-admit.
+Lemma updating_stripped_tree_is_inert''' : forall Γ tc ξ l t atypes x,
+         mapOptionTree (scbwv_ξ(Γ:=Γ)(tc:=tc)(atypes:=atypes) x ξ l)
+           (stripOutVars (vec2list (scbwv_exprvars x)) t)
+             =
+         mapOptionTree (weakLT' ○ ξ)
+           (stripOutVars (vec2list (scbwv_exprvars x)) t).
+  intros.
+  unfold scbwv_ξ.
+  unfold scbwv_varstypes.
+  admit.
   Qed.
-
-(*
-Lemma updating_stripped_tree_is_inert'''
-  {Γ}
-  (ξ:VV -> LeveledHaskType Γ)
-{T}
-  (idx:Tree ??T) (types:ShapedTree (LeveledHaskType Γ) idx)(vars:ShapedTree VV idx) tree
-:
-    mapOptionTree   (update_ξ''' ξ types vars) (stripOutVars (leaves (unshape vars)) tree)
-  = mapOptionTree ξ (stripOutVars (leaves (unshape vars)) tree).
-admit.
-  Qed.
-*)
 
 (* IDEA: use multi-conclusion proofs instead *)
 Inductive LetRecSubproofs Γ Δ ξ lev : forall tree, ELetRecBindings Γ Δ ξ lev tree -> Type := 
   | lrsp_nil  : LetRecSubproofs Γ Δ ξ lev [] (ELR_nil _ _ _ _)
-  | lrsp_leaf : forall v  e,
-    (ND Rule [] [Γ > Δ > mapOptionTree ξ (expr2antecedent e) |- [unlev (ξ v) @@ lev]]) ->
-    LetRecSubproofs Γ Δ ξ lev [(v, unlev (ξ v))] (ELR_leaf _ _ _ _ _ e)
+  | lrsp_leaf : forall v t e ,
+    (ND Rule [] [Γ > Δ > mapOptionTree ξ (expr2antecedent e) |- [t@@lev]]) ->
+    LetRecSubproofs Γ Δ ξ lev [(v, t)] (ELR_leaf _ _ _ _ _ t e)
   | lrsp_cons : forall t1 t2 b1 b2,
     LetRecSubproofs Γ Δ ξ lev t1 b1 ->
     LetRecSubproofs Γ Δ ξ lev t2 b2 ->
     LetRecSubproofs Γ Δ ξ lev (t1,,t2) (ELR_branch _ _ _ _ _ _ b1 b2).
 
-Lemma cheat1 : forall Γ Δ ξ lev tree (branches:ELetRecBindings Γ Δ ξ lev tree),
-  eLetRecTypes branches =
-    mapOptionTree  (update_ξ'' ξ tree lev)
-    (mapOptionTree (@fst _ _) tree).
-  intros.
-  induction branches.
-  reflexivity.
-  simpl.
-  unfold update_ξ.
-  unfold mapOptionTree; simpl.
-admit.
-admit.
-  Qed.
-Lemma cheat2 : forall Γ Δ ξ l tc tbranches atypes e alts',
-mapOptionTree ξ (expr2antecedent (ECase Γ Δ ξ l tc tbranches atypes e alts'))
-= 
-(*
-((mapOptionTreeAndFlatten
-(fun h => stripOutVars (vec2list (scbwv_exprvars (projT1 h)))
-                  (expr2antecedent (projT2 h))) alts'),,(expr2antecedent e)).
-*)
-((mapOptionTreeAndFlatten pcb_freevars
-           (mapOptionTree mkProofCaseBranch alts')),,mapOptionTree ξ  (expr2antecedent e)).
-admit.
-Qed.
-Lemma cheat3 : forall {A}{B}{f:A->B} l, unleaves (map f l) = mapOptionTree f (unleaves l).
-  admit.
-  Qed.
-Lemma cheat4 : forall {A}(t:list A), leaves (unleaves t) = t.
-admit.
-Qed.
-
-Lemma letRecSubproofsToND Γ Δ ξ lev tree branches
-    : LetRecSubproofs Γ Δ ξ lev tree branches ->
-    ND Rule []
-    [ Γ > Δ >
-      mapOptionTree ξ (eLetRecContext branches)
-      |-
-  eLetRecTypes branches
-    ].
-  intro X.
-  induction X; intros; simpl in *.
+Lemma letRecSubproofsToND Γ Δ ξ lev tree branches :
+  LetRecSubproofs Γ Δ ξ lev tree branches ->
+    ND Rule [] [ Γ > Δ > mapOptionTree ξ (eLetRecContext branches)
+      |- eLetRecTypes branches @@@ lev ].
+  intro X; induction X; intros; simpl in *.
     apply nd_rule.
       apply REmptyGroup.
     set (ξ v) as q in *.
       destruct q.
       simpl in *.
-      assert (h0=lev).
-        admit.
-        rewrite H.
       apply n.
     eapply nd_comp; [ idtac | eapply nd_rule; apply RBindingGroup ].
     eapply nd_comp; [ apply nd_llecnac | idtac ].
     apply nd_prod; auto.
   Defined.
 
-
-Lemma update_twice_useless : forall Γ (ξ:VV -> LeveledHaskType Γ ★) tree z lev,
-  mapOptionTree (@update_ξ'' Γ ξ tree lev) z = mapOptionTree (update_ξ'' (update_ξ'' ξ tree lev) tree lev) z.
-admit.
-  Qed.
-
-
-
 Lemma letRecSubproofsToND' Γ Δ ξ lev τ tree  :
     forall branches body,
-    ND Rule [] [Γ > Δ > mapOptionTree (update_ξ'' ξ tree lev) (expr2antecedent body) |- [τ @@ lev]] -> 
-    LetRecSubproofs Γ Δ (update_ξ'' ξ tree lev) lev tree branches ->
+    ND Rule [] [Γ > Δ > mapOptionTree (update_ξ ξ lev (leaves tree)) (expr2antecedent body) |- [τ @@ lev]] -> 
+    LetRecSubproofs Γ Δ (update_ξ ξ lev (leaves tree)) lev tree branches ->
     ND Rule [] [Γ > Δ > mapOptionTree ξ (expr2antecedent (@ELetRec VV _ Γ Δ ξ lev τ tree branches body)) |- [τ @@ lev]].
 
   (* NOTE: how we interpret stuff here affects the order-of-side-effects *)
-  simpl.
   intro branches.
   intro body.
   intro pf.
   intro lrsp.
-  set ((update_ξ ξ
-           (map (fun x : VV * HaskType Γ ★ => ⟨fst x, snd x @@  lev ⟩)
-              (leaves tree)))) as ξ' in *.
+  set ((update_ξ ξ lev (leaves tree))) as ξ' in *.
   set ((stripOutVars (leaves (mapOptionTree (@fst _ _) tree)) (eLetRecContext branches))) as ctx.
   set (mapOptionTree (@fst _ _) tree) as pctx.
   set (mapOptionTree ξ' pctx) as passback.
-  set (fun a b => @RLetRec Γ Δ a b passback) as z.
+  set (fun a b => @RLetRec Γ Δ a b (mapOptionTree (@snd _ _) tree)) as z.
   eapply nd_comp; [ idtac | eapply nd_rule; apply z ].
   clear z.
 
@@ -515,68 +486,99 @@ Lemma letRecSubproofsToND' Γ Δ ξ lev τ tree  :
 
   unfold ξ' in *.
   set (@updating_stripped_tree_is_inert') as zz.
-  unfold update_ξ'' in *.
   rewrite zz in q'.
   clear zz.
   clear ξ'.
-  simpl in q'.
-
+  Opaque stripOutVars.
+  simpl.
+  rewrite <- mapOptionTree_compose in q'.
+  cut ((mapOptionTree (update_ξ ξ lev (leaves tree) ○ (@fst _ _)) tree) = (mapOptionTree (@snd _ _) tree @@@ lev)).
+  intro H'.
+  rewrite <- H'.
   eapply nd_comp; [ idtac | apply q' ].
+  clear H'.
   clear q'.
-  unfold mapOptionTree. simpl. fold (mapOptionTree (update_ξ'' ξ tree lev)).
-
   simpl.
 
   set (letRecSubproofsToND _ _ _ _ _ branches lrsp) as q.
-
     eapply nd_comp; [ idtac | eapply nd_rule; apply RBindingGroup ].
     eapply nd_comp; [ apply nd_llecnac | idtac ].
     apply nd_prod; auto.
-    rewrite cheat1 in q.
-    set (@update_twice_useless Γ ξ tree ((mapOptionTree (@fst _ _) tree)) lev) as zz.
-    unfold update_ξ'' in *.
-    rewrite <- zz in q.
+    cut ((eLetRecTypes branches @@@ lev) = mapOptionTree (update_ξ ξ lev (leaves tree) ○ (@fst _ _)) tree).
+      intro H''.
+      rewrite <- H''.
     apply q.
+  admit.
+  admit.
+  admit.
   Defined.
 
-
-Lemma updating_stripped_tree_is_inert''' : forall Γ tc ξ l t atypes x,
-         mapOptionTree (scbwv_ξ(Γ:=Γ)(tc:=tc)(atypes:=atypes) x ξ l)
-           (stripOutVars (vec2list (scbwv_exprvars x)) t)
-             =
-         mapOptionTree (weakLT' ○ ξ)
-           (stripOutVars (vec2list (scbwv_exprvars x)) t).
+Lemma update_ξ_lemma `{EQD_VV:EqDecidable VV} : forall Γ ξ (lev:HaskLevel Γ)(varstypes:list (VV*_)),
+  distinct (map (@fst _ _) varstypes) ->
+  map (update_ξ ξ lev varstypes) (map (@fst _ _) varstypes) =
+  map (fun t => t@@ lev) (map (@snd _ _) varstypes).
+  intros.
+  induction varstypes.
+  reflexivity.
+  destruct a.
+  inversion H.
+  subst.
   admit.
   Qed.
 
+Lemma fst_zip : forall T Q n (v1:vec T n)(v2:vec Q n), vec_map (@fst _ _) (vec_zip v1 v2) = v1.
+  admit.
+  Qed.
 
-Lemma updating_stripped_tree_is_inert'''' : forall Γ Δ ξ l tc atypes tbranches 
-(x:StrongCaseBranchWithVVs(Γ:=Γ) VV eqd_vv tc atypes)
-(e0:Expr (sac_Γ x Γ) (sac_Δ x Γ atypes (weakCK'' Δ)) 
-    (scbwv_ξ x ξ l) (weakT' tbranches @@  weakL' l)) ,
-mapOptionTree (weakLT' ○ ξ)
-        (stripOutVars (vec2list (scbwv_exprvars x)) (expr2antecedent e0)),,
-unleaves (vec2list (sac_types x Γ atypes)) @@@ weakL' l
-=
-mapOptionTree (weakLT' ○ ξ)
-        (stripOutVars (vec2list (scbwv_exprvars x)) (expr2antecedent e0)),,
-         mapOptionTree
-           (update_ξ (weakLT' ○ ξ)
-              (vec2list
-                 (vec_map
-                    (fun
-                       x0 : VV *
-                            HaskType
-                              (app (vec2list (sac_ekinds x)) Γ)
-                              ★ => ⟨fst x0, snd x0 @@  weakL' l ⟩)
-                    (vec_zip (scbwv_exprvars x)
-                       (sac_types x Γ atypes)))))
-           (unleaves (vec2list (scbwv_exprvars x)))
-.
-admit.
-Qed.
+Lemma snd_zip : forall T Q n (v1:vec T n)(v2:vec Q n), vec_map (@snd _ _) (vec_zip v1 v2) = v2.
+  admit.
+  Defined.
 
+Lemma vec2list_injective : forall T n (v1 v2:vec T n), vec2list v1 = vec2list v2 -> v1 = v2.
+  admit.
+  Defined.
 
+Lemma scbwv_coherent {tc}{Γ}{atypes:IList _ (HaskType Γ) _} :
+  forall scb:StrongCaseBranchWithVVs _ _ tc atypes,
+    forall l ξ, vec_map (scbwv_ξ scb ξ l) (scbwv_exprvars scb) =
+                                 vec_map (fun t => t @@ weakL' l) (sac_types (scbwv_sac scb) _ atypes).
+  intros.
+  unfold scbwv_ξ.
+  unfold scbwv_varstypes.
+  set (@update_ξ_lemma _ _ (weakLT' ○ ξ) (weakL' l)
+    (vec2list (vec_zip (scbwv_exprvars scb) (sac_types (scbwv_sac scb) Γ atypes)))) as q.
+  rewrite vec2list_map_list2vec in q.
+  rewrite fst_zip in q.
+  rewrite vec2list_map_list2vec in q.
+  rewrite vec2list_map_list2vec in q.
+  rewrite snd_zip in q.
+  rewrite vec2list_map_list2vec in q.
+  apply vec2list_injective.
+  apply q.
+  apply scbwv_exprvars_distinct.
+  Qed.
+
+Lemma case_lemma : forall Γ Δ ξ l tc tbranches atypes e alts',
+  mapOptionTree ξ (expr2antecedent (ECase Γ Δ ξ l tc tbranches atypes e alts'))
+  = ((mapOptionTreeAndFlatten pcb_freevars (mapOptionTree mkProofCaseBranch alts')),,mapOptionTree ξ  (expr2antecedent e)).
+  intros.
+  simpl.
+  Ltac hack := match goal with [ |- ?A,,?B = ?C,,?D ] => assert (A=C) end.
+  hack.
+  induction alts'.
+  simpl.
+  destruct a.
+  unfold mkProofCaseBranch.
+  simpl.
+  reflexivity.
+  reflexivity.
+  simpl.
+  rewrite IHalts'1.
+  rewrite IHalts'2.
+  reflexivity.
+  rewrite H.
+  reflexivity.
+  Qed.
 
 
 Definition expr2proof  :
@@ -595,14 +597,14 @@ Definition expr2proof  :
     | ELet     Γ Δ ξ tv t      v lev ev ebody       => let case_ELet := tt in 
                                                        (fun pf_let pf_body => _) (expr2proof _ _ _ _ ev) (expr2proof _ _ _ _ ebody) 
     | ELetRec  Γ Δ ξ lev t tree branches ebody      =>
-      let ξ' := update_ξ'' ξ tree lev in
+      let ξ' := update_ξ ξ lev (leaves tree) in
       let case_ELetRec := tt in  (fun e' subproofs => _) (expr2proof _ _ _ _ ebody) 
-((fix subproofs Γ'' Δ'' ξ'' lev'' (tree':Tree ??(VV * HaskType Γ'' ★))
+        ((fix subproofs Γ'' Δ'' ξ'' lev'' (tree':Tree ??(VV * HaskType Γ'' ★))
         (branches':ELetRecBindings Γ'' Δ'' ξ'' lev'' tree')
         : LetRecSubproofs Γ'' Δ'' ξ'' lev'' tree' branches' :=
         match branches' as B in ELetRecBindings G D X L T return LetRecSubproofs G D X L T B with
           | ELR_nil    Γ Δ ξ lev  => lrsp_nil _ _ _ _
-          | ELR_leaf   Γ Δ ξ l v e => lrsp_leaf Γ Δ ξ l v e (expr2proof _ _ _ _ e)
+          | ELR_leaf   Γ Δ ξ l v t e => lrsp_leaf Γ Δ ξ l v t e (expr2proof _ _ _ _ e)
           | ELR_branch Γ Δ ξ lev t1 t2 b1 b2 => lrsp_cons _ _ _ _ _ _ _ _ (subproofs _ _ _ _ _ b1) (subproofs _ _ _ _ _ b2)
         end
         ) _ _ _ _ tree branches)
@@ -624,13 +626,17 @@ Definition expr2proof  :
                                    (weakLT' (tbranches@@l)) })
           : ND Rule [] (mapOptionTree (pcb_judg ○ mkProofCaseBranch) alts) :=
         match alts as ALTS return ND Rule [] (mapOptionTree (pcb_judg ○ mkProofCaseBranch) ALTS) with
-          | T_Leaf None       => let case_nil := tt in _
-          | T_Leaf (Some x)   => (fun ecb' => let case_leaf := tt in _) (expr2proof _ _ _ _ (projT2 x))
+          | T_Leaf None      => let case_nil := tt in _
           | T_Branch b1 b2   => let case_branch := tt in (fun b1' b2' => _) (mkdcsp b1) (mkdcsp b2)
+          | T_Leaf (Some x)  =>
+            match x as X return ND Rule [] [(pcb_judg ○ mkProofCaseBranch) X] with
+            existT scbx ex =>
+            (fun e' => let case_leaf := tt in _) (expr2proof _ _ _ _ ex)
+        end
         end) alts')
         in let case_ECase := tt in (fun e' => _) (expr2proof _ _ _ _ e)
     end
-); clear exp ξ' τ' Γ' Δ' expr2proof; try clear mkdcsp.
+  ); clear exp ξ' τ' Γ' Δ' expr2proof; try clear mkdcsp.
 
     destruct case_EGlobal.
       apply nd_rule.
@@ -659,12 +665,12 @@ Definition expr2proof  :
     destruct case_ELam; intros.
       unfold mapOptionTree; simpl; fold (mapOptionTree ξ).
       eapply nd_comp; [ idtac | eapply nd_rule; apply RLam ].
-      set (update_ξ ξ ((v,t1@@lev)::nil)) as ξ'.
+      set (update_ξ ξ lev ((v,t1)::nil)) as ξ'.
       set (arrangeContextAndWeaken v (expr2antecedent e) Γ Δ [t2 @@ lev] ξ') as pfx.
         apply UND_to_ND in pfx.
         unfold mapOptionTree in pfx; simpl in pfx; fold (mapOptionTree ξ) in pfx.
         unfold ξ' in pfx.
-        fold (mapOptionTree (update_ξ ξ ((v,(t1@@lev))::nil))) in pfx.
+        fold (mapOptionTree (update_ξ ξ lev ((v,t1)::nil))) in pfx.
         rewrite updating_stripped_tree_is_inert in pfx.
         unfold update_ξ in pfx.
         destruct (eqd_dec v v).
@@ -685,7 +691,7 @@ Definition expr2proof  :
       clear pf_body.
       fold (@mapOptionTree VV).
       fold (mapOptionTree ξ).
-      set (update_ξ ξ ((lev,(tv @@ v))::nil)) as ξ'.
+      set (update_ξ ξ v ((lev,tv)::nil)) as ξ'.
       set (arrangeContextAndWeaken lev (expr2antecedent ebody) Γ Δ [t@@v] ξ') as n.
       unfold mapOptionTree in n; simpl in n; fold (mapOptionTree ξ') in n.
       unfold ξ' in n.
@@ -739,28 +745,33 @@ Definition expr2proof  :
       apply e'.
 
     destruct case_leaf.
-      unfold pcb_judg.
+      clear o x alts alts' e.
+      eapply nd_comp; [ apply e' | idtac ].
+      clear e'.
+      set (existT
+              (fun scb : StrongCaseBranchWithVVs VV eqd_vv tc atypes =>
+               Expr (sac_Γ scb Γ) (sac_Δ scb Γ atypes (weakCK'' Δ))
+                 (scbwv_ξ scb ξ l) (weakLT' (tbranches @@  l))) scbx ex) as stuff.
+      set (fun q r x1 x2 y1 y2 => @UND_to_ND q r [q >> r > x1 |- y1] [q >> r > x2 |- y2]).
+      simpl in n.
+      apply n.
+      clear n.
+
+      rewrite mapleaves'.
       simpl.
-      repeat rewrite <- mapOptionTree_compose in *.
-      set (nd_comp ecb' (UND_to_ND _ _ _ _ (@arrangeContextAndWeaken'' _ _ _
-        (unleaves (vec2list (scbwv_exprvars (projT1 x))))
-      (*(unleaves (vec2list (sac_types (projT1 x) Γ atypes)))*)
-        _ _
-      ))) as q.
-      rewrite cheat4 in q.
-      rewrite cheat3.
-      unfold weakCK'' in q.
-      simpl in q.
-      rewrite (updating_stripped_tree_is_inert''' Γ tc ξ l _ atypes  (projT1 x)) in q.
-      Ltac cheater Q :=
-       match goal with
-        [ Q:?Y |- ?Z ] =>
-         assert (Y=Z) end.
-      cheater q.
-      admit.
-      rewrite <- H.
-      clear H.
-      apply q.
+      rewrite <- mapOptionTree_compose.
+      rewrite <- updating_stripped_tree_is_inert''' with (l:=l).
+      replace (vec2list (scbwv_exprvars scbx)) with (leaves (unleaves (vec2list (scbwv_exprvars scbx)))).
+      rewrite <- mapleaves'.
+      rewrite vec2list_map_list2vec.
+      unfold sac_Γ.      
+      rewrite <- (scbwv_coherent scbx l ξ).
+      rewrite <- vec2list_map_list2vec.
+      rewrite mapleaves'.
+      apply arrangeContextAndWeaken''.
+      rewrite leaves_unleaves.
+      apply (scbwv_exprvars_distinct scbx).
+      apply leaves_unleaves.
 
     destruct case_nil.
       apply nd_id0.
@@ -772,18 +783,19 @@ Definition expr2proof  :
       apply b2'.
 
     destruct case_ECase.
-      rewrite cheat2.
+      rewrite case_lemma.
       eapply nd_comp; [ idtac | eapply nd_rule; eapply RCase ].
       eapply nd_comp; [ apply nd_llecnac | idtac ]; apply nd_prod.
       rewrite <- mapOptionTree_compose.
       apply dcsp.
       apply e'.
 
-    destruct case_ELetRec; simpl in *; intros.
-      set (@letRecSubproofsToND') as q.
-      simpl in q.
-      apply q.
-      clear q.
+    destruct case_ELetRec; intros.
+      unfold ξ'0 in *.
+      clear ξ'0.
+      unfold ξ'1 in *.
+      clear ξ'1.
+      apply letRecSubproofsToND'.
       apply e'.
       apply subproofs.
 
